src/riscv/Proofs/VerifyDecode.v
@@ -1,0 +1,108 @@
+Require Export Coq.ZArith.ZArith.
+Require Export Coq.Lists.List. Import ListNotations.
+Require Import coqutil.Tactics.rdelta.
+Require Import coqutil.Tactics.destr.
+Require Import coqutil.Z.prove_Zeq_bitwise.
+Require Import coqutil.Tactics.Tactics.
+Require Import coqutil.Tactics.fwd.
+Require Export riscv.Spec.Decode.
+Require Export riscv.Utility.Encode.
+Require Export riscv.Utility.Utility.
+Require Import riscv.Proofs.DecodeByExtension.
+
+Local Open Scope Z_scope.
+
+Ltac isConst x :=
+  lazymatch x with
+  | ?a ^ ?b => isConst a; isConst b
+  | ?a - ?b => isConst a; isConst b
+  | - ?a => isConst a
+  | Z.max ?a ?b => isConst a; isConst b
+  | _ => let x' := rdelta x in
+         lazymatch isZcst x' with
+         | true => idtac
+         end
+  end.
+
+Lemma verify_decode: forall iset inst,
+    supportsF iset = false ->
+    verify (decode iset inst) iset \/ decode iset inst = InvalidInstruction inst.
+Proof.
+  intros. rewrite <- decode_seq_correct.
+  assert (bitwidth iset = 2 ^ 5 \/ bitwidth iset = 2 ^ 6) as bw_cases. {
+    destruct iset; cbn; auto.
+  }
+  assert (bitSlice inst 25 26 = 0 -> bitSlice inst 20 26 < bitwidth iset). {
+    intros.
+    rewrite bitSlice_alt in *. 2-3: cbv; intuition congruence.
+    unfold bitSlice' in *.
+    Z.div_mod_to_equations.
+    Lia.lia.
+  }
+  assert (signExtend 32 (BinInt.Z.shiftl (bitSlice inst 12 32) 12) mod 2 ^ 12 = 0). {
+    unfold signExtend.
+    rewrite Z.shiftl_mul_pow2 by (cbv; discriminate 1).
+    Z.div_mod_to_equations.
+    Lia.lia.
+  }
+  assert (signExtend 13
+   (Z.shiftl (bitSlice inst 31 32) 12 <|> BinInt.Z.shiftl (bitSlice inst 25 31) 5 <|>
+    Z.shiftl (bitSlice inst 8 12) 1 <|> BinInt.Z.shiftl (bitSlice inst 7 8) 11) mod 2 = 0). {
+    eapply mod20_bitSlice.
+    prove_Zeq_bitwise.
+  }
+  assert (signExtend 21
+   (BinInt.Z.shiftl (bitSlice inst 31 32) 20 <|> BinInt.Z.shiftl (bitSlice inst 21 31) 1 <|>
+    BinInt.Z.shiftl (bitSlice inst 20 21) 11 <|> BinInt.Z.shiftl (bitSlice inst 12 20) 12)
+   mod 2 = 0). {
+    eapply mod20_bitSlice.
+    prove_Zeq_bitwise.
+  }
+  unfold decode_seq.
+  repeat destruct_one_match; fwd.
+  all: (right; reflexivity) || left.
+  all: try match goal with
+           | H': supportsF _ = true |- _ => exfalso; congruence
+           end.
+  all: unfold verify, verify_iset.
+  all: split;
+    [|repeat match goal with
+             | H: bitwidth _ = _ |- _ => unfold bitwidth in H
+             end;
+      unfold supportsM, supportsA, supportsF in *;
+      destruct iset; try intuition congruence].
+  all: match goal with
+       | |- respects_bounds _ (_ ?d) => remember d as r in *; revert dependent r; intro r
+       end.
+  all: cbv beta zeta delta [decodeI decodeM decodeA decodeF
+                            decodeI64 decodeM64 decodeA64 decodeF64
+                            decodeCSR
+                            isValidI isValidM isValidA isValidF
+                            isValidI64 isValidM64 isValidA64 isValidF64
+                            isValidCSR].
+  all: loop INil.
+  all: intros; subst.
+  all: match goal with
+       | H: ?x = ?x |- _ => clear H
+       | H: false = true |- _ => discriminate H
+       end.
+  all: cbv beta iota zeta delta [respects_bounds apply_InstructionMapper Verifier
+         map_Invalid map_R map_R_atomic map_I map_I_shift_57 map_I_shift_66
+         map_I_system map_S map_SB map_U map_UJ map_Fence map_FenceI
+         verify_Invalid verify_R verify_R_atomic verify_I verify_I_shift_57 verify_I_shift_66
+         verify_I_system verify_S verify_SB verify_U verify_UJ verify_Fence verify_FenceI
+         machineIntToShamt id
+       ].
+  all: repeat match goal with
+              | |- 0 <= bitSlice _ _ _ < _ => eapply bitSlice_bounds
+              | |- _ <= signExtend _ _ < _ => eapply signExtend_bounds; cbv; discriminate 1
+              | |- _ /\ _ => split
+              | |- ?x <= ?y => isConst x; isConst y; cbv; discriminate 1
+              | |- ?x < ?y => isConst x; isConst y; reflexivity
+              | |- 0 <= bitSlice _ _ _ => eapply bitSlice_nonneg
+              | |- bitSlice _ _ _ < 2 ^ _ => eapply bitSlice_upper_bound
+              | |- _ < bitwidth ?iset => replace (bitwidth iset) with 64;
+                                         [ change 64 with (2 ^ 6) ]
+              | |- _ => auto 3
+              end.
+Qed.
